theory/InterpreterSafety.thy
@@ -1,0 +1,15 @@
+section \<open> The Safety proof of the Interpreter in Solana rBPF \<close>
+
+theory InterpreterSafety
+imports
+  Main
+  rBPFCommType rBPFSyntax vm_state vm Mem
+  ebpf rBPFDecoder
+  verifier Interpreter
+begin
+  
+lemma interpreter_safe: "verifier l sv fm cb = True \<Longrightarrow>
+  bpf_interp fuel l (BPF_OK pc rs m ss sv fm cur_cu remain_cu) eb \<noteq> BPF_Err"
+
+
+end
