theory/Interpreter_Code_Gen.thy
@@ -1,0 +1,28 @@
+theory Interpreter_Code_Gen
+imports
+  Main
+  rBPFCommType rBPFSyntax vm_state vm Mem
+  ebpf rBPFDecoder Interpreter
+begin
+
+definition init_rs :: "reg_map" where
+"init_rs r = 0"
+
+definition test_eval_reg :: "u64" where
+"test_eval_reg = eval_reg BR0 init_rs"
+
+definition test_prog :: "int list \<Rightarrow> int" where
+"test_prog l = 1"
+
+code_printing
+  type_constructor nat \<rightharpoonup> (OCaml) "nat"
+code_printing
+  type_constructor int \<rightharpoonup> (OCaml) "int"
+
+declare [[code abort: storev loadv]]
+(*
+export_code eval_reg in OCaml
+  module_name Test_eval_reg file \<open>test_eval_reg.ml\<close>
+*)
+
+end
