theory/Mem.thy
@@ -8,13 +8,23 @@ begin
 
 type_synonym mem = "(u64, u8 option) map"
 
+definition init_mem :: "mem" where
+"init_mem = (\<lambda> _. None)"
+
 datatype memory_chunk = M8 | M16 | M32 | M64
 
-type_synonym addr_type = val
+type_synonym addr_type = u64
 
 axiomatization
   loadv   :: "memory_chunk \<Rightarrow> mem \<Rightarrow> addr_type \<Rightarrow> val option" and
   storev  :: "memory_chunk \<Rightarrow> mem \<Rightarrow> addr_type \<Rightarrow> val \<Rightarrow> mem option"
+
+(*
+definition load :: "memory_chunk \<Rightarrow> mem \<Rightarrow> addr_type \<Rightarrow> val option" where
+"load mc m addr = (
+  case mc of
+  M8 \<Rightarrow> 
+)" *)
 
 definition vlong_of_memory_chunk :: "memory_chunk \<Rightarrow> val" where
 "vlong_of_memory_chunk chunk = (
